<?xml version="1.0" encoding="UTF-8"?>

<section xml:id="sec-exp-intro" xmlns:xi="http://www.w3.org/2001/XInclude">
  <title>Exponential Rules</title>
  
  <objectives>
	<ul>
		<li>
			<p>
				Use exponent rules to simplify and re-work expressions.
			</p>
		</li>
		<li>
			<p>
				Simplify roots/radicals without a calculator. 
			</p>
		</li>
		<li>
			<p>
				Avoid common errors regarding exponents and radicals.
			</p>
		</li>
	</ul>
</objectives>
 
<assemblage xml:id="exp-use">
	<title>Where will this be used in calculus?</title>
	<p>
		Rewriting and simplifying exponentials and radicals is usefully in most computational areas of mathematics, including calculus. Here are two specific calculus examples: 

	<ul>
		<li>
			<p>
				When differentiating or integrating a power function (or a combination of power functions), rewrite each term as a single power before differentiating or integrating. For example, rewriting <m>f(x) = \frac{1}{x^4}</m> as <m>f(x) = x^{-4}</m> will make it easier to differentiate or integrate. 
			</p>
		</li>
		<li>
			<p>
				After using rules to differentiate a function (for example the product rule, quotient rule or chain rule) the result is often a messy complicated looking expression which needs to be simplified. 
			</p>
		</li>
	</ul>
</p>
</assemblage>

 
  <introduction>
    <!--<p> Before we dive into the different rules, we need to have a solid understanding of what exponents are and what they mean.   </p>
	<p>
		When we first start learning math, we often start with addition. We then quickly see that repeated addition can be useful. We run into problems like: ``You have 4 dogs and want to give each dog 3 treats. How many treats do you need?'' We solve these with repeated addition: <m>3+3+3+3 = 12</m>, or three treats for each of the four dogs. We then learn that repeated addition happens often, so we develop a new notation, multiplication. For our example problem, we would do <m>3 \times 4</m> to say we need to add three, four times. Exponents take this one step further. When we need to do repeated multiplication, like if we need to find the volume of a cube, we can shorten the notation by using exponents. To find our volume, we would multiply the side length by itself three times to get length times width times height, but with a cube these lengths are all the same. We can write <m>V(x) = (x)(x)(x)=x^3</m>. Here, the exponent tells us how many times to do the multiplication. The concept can later be exanded to include non-integer values of the exponent. But starting by looking at integer exponents can give us an intuitive idea of what exponentials are and how to work with them. 
	</p>
   -->

  <p>
   As an instroduction, we can think of integer exponents as repeated multiplication. If we want to find the volume of a cube, we can shorten the notation by using exponents. To find the volume of a cube with side length <m> x </m>, we would multiply <m> x </m> by itself three times to get length times width times height. We can write <m>V(x) = (x)(x)(x)=x^3</m>. Here, the exponent tells us how many times to do the multiplication. The concept can later be <em> exanded to include non-integer values of the exponent </em>. But starting by looking at integer exponents can give us an intuitive idea of what exponentials are and how to work with them. 
  </p>
</introduction>

  <subsection>
	<title>The First Rules</title>
  <p>
  The first exponent rule we will examine is
  </p>
	<men xml:id="rule-one">
		x^ax^b=x^{a+b}.
	</men>

  <p>
  Here, the first term, <m>x^a</m> tells us to multiply <m>x</m> by itself <m>a</m> times and the second term tells us to multiply it <m>b</m> times. Together, that says we need to multiply <m>x</m> a total of <m>a+b</m> times, giving us <m>x^{a+b}</m>. As an example, <m>x^2x^3 = x^{2+3} = x^5</m>. 
  </p>
  
  <exercise xml:id="ex-exp-CP1">
	<webwork source="Library/PCC/BasicAlgebra/Exponents/exponentsMultiplication0.pg" />
  </exercise>

  <p> 
	Note that <xref ref="rule-one" /> is true for all real numbers <m>a</m> and <m>b</m> (they do not need to be integers), and all positive values of <m>x</m>.
  </p> 



  <p>  
  Next, let's look at
  </p>
<me> x^{-a} = \frac{1}{x^a}.</me>
  
 
  <p>
  This rule builds off of our previous rule. If we have <m>x^5x^{-2}</m>, rule <xref ref="rule-one" /> tells us that we really have <m>x^{5+(-2)} = x^{5-2} = x^3</m>. We went from having <m>x</m> multiplied 5 times to having <m>x</m> multiplied only 3 terms, meaning we have removed two of the multiplications. We removed a multiplication through a division: 
  </p>

  <md>
	<mrow>\frac{x^5}{x^2} &amp;= \frac{(x)(x)(x)(x)(x)}{(x)(x)}</mrow>
	<mrow> 		&amp;= (x)(x)(x)</mrow>
	<mrow> 		&amp;= x^3.</mrow>
</md>

<p>
  A negative exponent tells us we have division rather than multiplication. 
   <!--- We can also combine this rule with some of our rules from fractions. 
 If we have <m>\frac{1}{x^{-a}}</m>, we can start by replacing <m>x^{-a}</m> with <m>\frac{1}{x^a}</m>. This gives us
</p>

<me>
	\frac{1}{x^{-a}} = \frac{1}{\frac{1}{x^a}}. 
</me>

<p>
From our fractions rules, -->
<!---We know that dividing by a fraction is the same as multiplying by its reciprocal. We can use that to see
<md>
  <mrow>\frac{1}{x^{-a}} &amp;= \frac{1}{\frac{1}{x^a}}</mrow>
  <mrow> 		&amp;= 1 \times \frac{x^a}{1}</mrow>
  <mrow> 		&amp;= x^a.</mrow>
</md>.-->

A more general version of the rule is the following:
<men xml:id="rule-two"> 
	x^{b-a} = \frac{x^b}{x^a}.
</men>
We can see this from previous rules: 
<md>
	<mrow>x^{b-a} &amp;= x^{b}x^{-a}</mrow>
	<mrow> 		&amp;= x^{b} \times \frac{1}{x^a}</mrow>
	<mrow> 		&amp;= \frac{x^b}{x^a}.</mrow>
</md>

Again, all of the above is true for all real numbers <m>a</m> and <m>b</m>, and all positive values of <m>x</m>. 
</p>

  <exercise xml:id="ex-exp-numbers">
	<webwork source="Library/FortLewis/Basic-skills-pretest/Skill-Assessment-05.pg" />
  </exercise>
  <exercise xml:id="ex-exp-div">
	<webwork source="Library/PCC/BasicAlgebra/Exponents/negExp36.pg" />
  </exercise>
  <exercise xml:id="ex-exp-multdiv">
	<webwork source="Library/FortLewis/Algebra/6-1-Exponent-rules/MCH1-6-1-36-Exponent-rules.pg" />
  </exercise>

  <p>
If there are several different base numbers we need to collect those with the same base, as in the following example.
  </p>

  <example>
	<title>Simplifying exponents with several bases</title>
	<statement>
		Simplify the expression <m>(11x^5u^2)(7u^3x^4)</m>.
	</statement>
	<answer>
	  <p>
		<me>
			\boxed{(11x^5u^2)(7u^3x^4) = 77x^9u^5}
		</me>
	  </p>
	</answer>
	<solution>
		<p>
			We can multiply the constant coefficients (11 and 7):
		</p>
		<me>
			(11x^5u^2)(7u^3x^4) = 77(x^5u^2)(u^3x^4)
		</me>			
			
		<p>
			Next, we can use rule <xref ref="rule-one" /> to simplify powers of <m>x</m>, and then use <xref ref="rule-one" /> again for powers of <m>u</m>. 
		</p>
			<md>
					<mrow>77(x^5u^2)(u^3x^4) &amp;= 77(x^5x^4)(u^2u^3)</mrow>
					<mrow> 		&amp;= 77 \times x^{5+4} \times u^{2+3}</mrow>
					<mrow> 		&amp;= 77x^9u5.</mrow>
			</md>	
		<p>
			The final result is:
		</p>
		<me>
			\boxed{(11x^5u^2)(7u^3x^4) = 77x^9u^5}
		</me>
	</solution>
</example>




  <exercise xml:id="ex-exp-mult2">
	<webwork source="Library/CollegeOfIdaho/setAlgebra_01_06_Exponents/16IntAlg_28_Exponents.pg" />
  </exercise>
</subsection>

  <subsection>
	<title> Roots </title>

  <p>
	Before we continue with more exponent rules, let's look at the inverse function, or how to ``undo'' an exponent. These are root functions. A square root ``undoes'' squaring and a cube root ``undoes'' cubing. In general, we have
	</p>


	<me>
		(x^a)^{1/a} = x  
	</me>
	
	<p>
	and 
	</p>
	
	<me>
		(x^{1/a})^a = x
	</me>
	
	
	
	<p>
	(Both of the above are examples of rule <xref ref="rule-three" />, which we will look more at soon.) 
	</p>
		
	<p>
	Often, you will see <m>x^{1/a}</m> written as <m>\sqrt[a]{x}</m>. 
	Mathematicians call <m>\sqrt[a]{x}</m> the <term>radical</term> form and <m>x^{1/a}</m> the <term>exponential</term> form.
	
	Both have the same meaning. Anytime you see <m>\sqrt[a]{x}</m>, you can replace it with <m>x^{1/a}</m> and vice versa.
	<men>
		x^{1/a} = \sqrt[a]{x}
	</men>
	Even more generally, we have:
	<men>
		x^{b/a} = \sqrt[a]{x^b} = \left( \sqrt[a]{x} \right)^b
	</men>
	which is true for all real numbers <m>a</m> and <m>b</m>, and all positive values of <m>x</m>.
	</p>
	
	  <p>
		Sometimes it is useful to be able to simplify radicals or fractional exponents by hand. Let's take a look at how we can evaluate these types of terms.
		</p>
		
	
	<example>
		<title>Evaluating radicals</title>
		<statement>
			Evaluate <m>8^{2/3}</m> without using a calculator.
		</statement>
		<answer>
		  <p>
			<me>
				\boxed{8^{2/3} = 4}
			</me>
		  </p>
		</answer>
		<solution>
			As first glance, this looks like we won't be able to do much with it. However, we can use our exponent rules to help us evaluate it. We can rewrite this as <m>(8^2)^{1/3}</m> or as <m>(8^{1/3})^2</m>. We prefer the second version. With the first version we would have <m>(8^2)^{1/3} = (64)^{1/3}</m>, but this is tricky to deal with by hand because not many people have perfect cubes memorized, so we would need to factor <m>64</m>.
	
			<p>
			If we use the second version, <m>(8^{1/3})^2</m>, we would start by finding the cube root of 8. When we factor, we get <m>8=2\times2\times2</m>, which show us that <m>2=8^{1/3}</m>. This gives us <m>(8^{1/3})^2 = (2)^2 = 4</m>, so our final answer is
			</p>
			<me>
				\boxed{8^{2/3} = 4}
			</me>
		</solution>
	</example>
	


	  <exercise xml:id="ex-exp-root">
		<webwork source="Library/LoyolaChicago/Precalc/Chap3Tools/Connally3-3-Tools-28.pg" />
	  </exercise> 

	  <exercise>
		<webwork source="Library/UMN/algebraKaufmannSchwitters/ks_5_4_6.pg" />
	  </exercise> 

	  <exercise xml:id="ex-exp-root3">
		<webwork source="Library/UMN/algebraKaufmannSchwitters/ks_5_4_16.pg" />
	  </exercise> 
 
</subsection>

<subsection>
	<title> More exponential rules </title>
<p>
  The next rule we will discuss is
</p>
<equation>
  <men xml:id="rule-three">
	(x^a)^b = x^{ab}.
  </men>
</equation>


<p>
  This rule builds directly off of our first rule as well. As a example when <m>a</m> and <m>b</m> are integers, <m>(x^a)^b</m> tells us we need to multiply <m>x^a</m> by itself <m>b</m> times. Since <m>x^a</m> multiplies <m>x</m> by itself <m>a</m> times, <m>(x^a)^b</m> tells us to multiply <m>x</m> by itself a total of <m>ab</m> times. For example, 
</p>

<md>
	<mrow>(x^2)^3 &amp;= (x^2)(x^2)(x^2)</mrow>
	<mrow> 		&amp;= x^{2+2+2}</mrow>
	<mrow> 		&amp;= x^{2  \times 3}</mrow>
	<mrow> 		&amp;= x^6</mrow>
</md>

<p> 
	We can also use this rule when there is a product or quotient inside the parentheses, but not if there is an addition or subtraction. 
	
	<equation>
		<men xml:id="rule-four">
			(xy)^{a} = x^{a}y^{a}
		</men>
	  </equation>	
	  <equation>
		<men xml:id="rule-five">
			\left(\frac{x}{y}\right)^{a} = \frac{x^{a}}{y^{a}}
		</men>
	  </equation>	
However,
<equation>
	<me>
		(x+y)^a \not= x^a + y^a
	</me>
  </equation>
</p>

<example>
	<title>Double exponents</title>
	<statement>	
		Simplify <me>(x^2y^3)^2</me> and 
		<me> \Bigg(\frac{3x^2}{y^3}\Bigg) ^2</me>
	</statement>
	<answer>
	<p>
		<me>
			\boxed{(x^2y^3)^2 =x^4 y^6}
		</me>
		and 		<me>
			\boxed{(\Bigg(\frac{3x^2}{y^3}\Bigg) ^2 =\frac{9x^4}{y^6}}
		</me>
	  </p>
	</answer>
	<solution>	
		Using the rules we have seen above, we have that:
		<md>
			<mrow>(x^2y^3)^2 &amp;= (x^2)^2(y^3)^2 </mrow>
			<mrow> 		&amp;= x^4 y^6</mrow>
		</md>
		and 
		<md>
			<mrow>\Bigg (\frac{3x^2}{y^3}\Bigg) ^2 &amp;= \frac{(3x^2)^2}{(y^3)^2}</mrow>
			<mrow> 		&amp;= \frac{3^2(x^2)^2}{(y^3)^2}</mrow>
			<mrow> 		&amp;= \frac{9x^4}{y^6}</mrow>
		</md>
	</solution>
</example>

<example xml:id="ex-add">
	<title>Exponents and addition</title>
	<statement>	
		Are <m>(x^2+y^3)^2</m> and <m> x^4+y^6</m> equal of different? 
	</statement>
	<solution>	
		They are different. <m>(x^2+y^3)^2\not= x^4+y^6</m> in general. We can test this by chosing some values for <m>x</m> and <m>y</m>, then checking what the expressions are. For example, let <m>x=2</m> and <m> y=1</m>. Then <m>(x^2+y^3)^2=25</m> and <m> x^4+y^6 = 17</m> so they are not equal.
	</solution>
</example>

<example>
	<title>Addition inside a bracket</title>
	<statement>
	<p>
		Simpliy the expression <m>(x^2+y^3)^2</m>. 
	</p>
	</statement>

	<hint>
		<p>
			To simplify <m>(x^2+y^3)^2</m> we could rewrite it as <m>(x^2+y^3)(x^2+y^3)</m> and distribute. Or it would be even faster to use rule <m>(a+b)^2 = a^2 + 2ab + b^2</m>.
		</p>
	</hint>

	  <answer>
	  <p>
		<me>
			\boxed{(x^2+y^3)^2 = x^4 + 2x^2y^3 + y^6}
		</me>
	  </p>
	</answer>
	<solution>
		<p>
			To simplify <m>(x^2+y^3)^2</m> we can rewrite it as <m>(x^2+y^3)(x^2+y^3)</m> and distribute.
		</p>

		<md>
			<mrow>(x^2+y^3)^2 &amp;= (x^2+y^3)(x^2+y^3)</mrow>
			<mrow> 		&amp;= x^2 \times x^2 + x^2y^3 + y^3x^2+ y^3 y^3</mrow>
			<mrow> 		&amp;= x^4 + 2x^2y^3 + y^6.</mrow>
	</md>

		<me>
			\boxed{(x^2+y^3)^2 = x^4 + 2x^2y^3 + y^6}
		</me>
	</solution>
</example>

<exercise xml:id="ex-exp-radical2">
	<webwork source="Library/FortLewis/Algebra/6-2-Fractional-exponents/MCH1-6-2-04-Fractional-exponents.pg" />
  </exercise> 

	<exercise>
		<webwork source="Library/Mizzou/Algebra/exponents_rational/conv_exp_to_exp_two_term_mult_01.pg" />
	  </exercise> 

	  <exercise xml:id="ex-exp-div2">
		<webwork source="Library/CollegeOfIdaho/setAlgebra_01_06_Exponents/16IntAlg_34_Exponents.pg" />
	  </exercise> 

	  <exercise xml:id="ex-exp-radical3">
		<webwork source="Library/Mizzou/Algebra/radicals_simplifying/foiling_05.pg" />
	  </exercise> 

</subsection>

<subsection>
	<title>Summary</title>
<p>
The rules we have just seen will all be quite handy in calculus (and many other fields of mathematics, of course). In both integral and differential calculus, we will have rules that work well when we have a power function (a function of the form <m>f(x)=x^a</m>), but won't work for other forms of functions. By being able to rewrite functions like <m>f(x) = \frac{1}{x^4}</m>, in power function form (<m>f(x) = x^{-4}</m> in this case), other calculations will be simplified. 
</p>
<p>
Our rules are summarized below.
</p>

<assemblage xml:id="exp-rules">
	<title>Exponential Rules</title>
	<p>
		The following are true for all positive numbers <m>x</m> and <m>y</m>, and any real numbers <m>a</m> and <m>b</m>:
		<tabular>
		  <row>
			<cell>
				<me>x^ax^b=x^{a+b}</me>
			</cell>
			<cell>
				<m>\hspace{15mm}</m>
			</cell>
			<cell>
				<xref ref="rule-one" />
			</cell>
		  </row>
		  <row>
			<cell>
				<me>x^{a-b} = \frac{x^a}{x^b}</me>
			</cell>
			<cell>
				<m>\hspace{15mm}</m>
			</cell>
			<cell>
				<xref ref="rule-two" />
			</cell>
		  </row>
		  <row>
			<cell>
				<me>(x^a)^b = x^{ab}</me>
			</cell>
			<cell>
				<m>\hspace{15mm}</m>
			</cell>
			<cell>
				<xref ref="rule-three" />
			</cell>
		  </row>
		  <row>
			<cell>
				<me>(xy)^{a} = x^{a}y^{a}</me>
			</cell>
			<cell>
				<m>\hspace{15mm}</m>
			</cell>
			<cell>
				<xref ref="rule-four" />
			</cell>
		  </row>
		  <row>
			<cell>
				<me>\left(\frac{x}{y}\right)^{a} =\frac{x^a}{y^a}</me>
			</cell>
			<cell>
				<m>\hspace{15mm}</m>
			</cell>
			<cell>
				<xref ref="rule-five" />
			</cell>
		  </row>
		</tabular>
	</p>

</assemblage>

<assemblage xml:id="exp-notation">
	<title>Notation</title>
	<p>
		Suppose <m>x</m> is any positive number <m>x</m>, and <m>a</m> and <m>b</m> are integers, with <m>a>0</m>. Then:
			<ul>
				<li> <m>x^{1/a} = \sqrt[a]{x}</m> </li>
			</ul>
			<ul>
				<li> <m>x^{b/a} = \sqrt[a]{x^b} = \left( \sqrt[a]{x} \right)^b </m> </li>
			</ul>
	</p>
</assemblage>


<p>
	It is important to know mathematical rules and how to use them, but it is also important to know which `rules' are not true. Here are a few common errors:
</p>

<assemblage>
	<title>Common Errors</title>
	<p>
		The following expressions are not equal, in general.
		<men xml:id="error-one">(x+y)^2 \not= x^2 + y^2</men>
		<men xml:id="error-two">(x+y)^a \not= x^a + y^a</men>
		<men xml:id="error-three">\sqrt{x+y} \not= \sqrt{x} + \sqrt{y}</men>
		<men xml:id="error-four">x^{a}y^{b} \not= (xy)^{ab}</men>
		<men xml:id="error-five">\frac{x^a}{y^b} \not= \left(\frac{x}{y}\right)^{a-b} </men>
	</p>
</assemblage>
</subsection>

<subsection>
	<title>Additional Examples</title>
<p>
Let's look at a few examples of working with exponent rules. The examples use one or several of the rules we have seen above. 
</p>

<p>
<alert>You are strongly encouraged to try the examples first on your own, before looking at the worked solutions.</alert>
</p>

<example>
	<title>Simplifying exponents</title>
	<statement>
		<p>
		Simplify <me> \Bigg( \frac{x^2 y^4}{x\sqrt{y}}\Bigg)^2</me>
		</p>
	</statement>
	<answer>
		<p>
			<me>\boxed{\Bigg( \frac{x^2 y^4}{x\sqrt{y}}\Bigg)^2=x^2y^7}</me>
		</p>
	  </answer>
	<solution>
		<p>
		Anytime we simplify, we need to remember our order of operations. The order of operations tells us to start with terms that are inside of parentheses, so we will work on simplifying the fraction before we worry about the exponent on the outside. First, we will write everything using exponents rather than radicals so we can use our exponent rules more easily in the rest of the problem.
		</p>
		<me>
			\Bigg( \frac{x^2 y^4}{x\sqrt{y}}\Bigg)^2 = \Bigg( \frac{x^2 y^4}{xy^{1/2}}\Bigg)^2
		</me>
		<p>
		Next, we will eliminate the fraction by using negative exponents on the terms that are in the denominator. After rewriting, we will combine any like terms.
		</p>
		<md>
			<mrow>\Bigg( \frac{x^2 y^4}{xy^{1/2}}\Bigg)^2 &amp;= \Big( x^2 y^4 x^{-1} y^{-1/2} \Big)^2</mrow>
			<mrow> 		&amp;= \Big( x^2 x^{-1} y^4 y^{-1/2} \Big)^2</mrow>
			<mrow> 		&amp;= \Big( x^{2-1} y^{4-1/2} \Big)^2</mrow>
			<mrow> 		&amp;= \Big( x^1 y^{8/2-1/2}\Big)^2</mrow>
			<mrow> 		&amp;= \Big( x y^{7/2})^2</mrow>	
		</md>
		<p>
		Now that everything inside the parentheses is simplified as much as possible, we will use our third exponent rule to finish simplifying. Rule <xref ref="rule-three"/> says that <m>(x^a)^b = x^{ab}</m>. We need to make sure we distribute the exponent that is outside of the parentheses to each term inside of the parentheses. This give us
		</p>

		<md>
			<mrow>\Big( x y^{7/2}\Big)^2 &amp;= (x)^2 (y^{7/2})^2</mrow>
			<mrow> 		&amp;= x^2 y^{14/2}</mrow>
			<mrow> 		&amp;= x^2y^7</mrow>
		</md>

		<p>
		So, in the end, we get that
		<me>\boxed{\Bigg( \frac{x^2 y^4}{x\sqrt{y}}\Bigg)^2=x^2y^7}</me>
		</p>
	</solution>
</example>

<example>
	<title>Simplifying exponents involving addition</title>
	<statement>
		Simplify <me>\displaystyle \Big( \sqrt{y} + \sqrt{x}\Big)^2.</me>
	</statement>
	<answer>
		<p>
		  <me>
			\boxed{\Big( \sqrt{y} + \sqrt{x}\Big)^2 = y + 2\sqrt{yx} + x}
		  </me>
		</p>
	  </answer>
	<solution>
		<p>
		Note: Be careful to avoid the common error <xref ref="error-one" /> above.
		</p>


		<p>
		We'll start by focusing on the terms inside the parentheses and rewriting all radicals (roots) as exponents. This gives us
			<me>
				\Big( \sqrt{y} + \sqrt{x} \Big)^2 = \Big( y^{1/2} + x^{1/2} \Big)^2.
			</me>
		There is nothing that we can simplify inside the parentheses. We now need to apply the exponent on the outside of the parentheses. Inside the parentheses we have two terms that are added, so we can't apply an exponent rule here. We will need to rewrite and then expand.
		<md>
			<mrow>\Big(y^{1/2} + x^{1/2} \Big)^2 &amp;= \Big(y^{1/2} + x^{1/2} \Big)\Big(y^{1/2} + x^{1/2} \Big)</mrow>
			<mrow> 		&amp;= (y^{1/2})^2 + 2 y^{1/2}x^{1/2} + (x^{1/2})^2</mrow>
			<mrow> 		&amp;= y + 2 y^{1/2}x^{1/2} + x</mrow>
		</md>.
		We don't have any like terms, so we can't simplify any further. We could rewrite slightly, but this is a matter of personal preference. We have three other ways we could write this final answer. We could use exponent rules to rewrite the middle term since <m>y^{1/2}x^{1/2}=(yx)^{1/2}</m>, giving us <m>y+2(yx)^{1/2} + x</m>. We could also use radicals and write either <m>y + 2\sqrt{y}\sqrt{x} + x</m> or <m>y+2\sqrt{yx} + x</m>. All of these four answers are fully simplified, and are equally valid. Probably the most common form is
		<me>
			\boxed{\Big( \sqrt{y} + \sqrt{x}\Big)^2 = y + 2\sqrt{yx} + x}
		</me>
	</p>

	</solution>
</example>
</subsection>




<subsection>
	<title>Mixed Exercises</title>
<p>
	1. Look at each of the "common errors" listed above. For each one, explain why it is not true. Replace the letters with numbers (choose some numbers!), to check that often the two sides are not equal, similar to the solution of <xref ref="ex-add"/>. 
</p>

<p>
	2. <webwork source="Library/FortLewis/Algebra/6-1-Exponent-rules/MCH1-6-1-14-Exponent-rules.pg" />
</p>

<p>
	3.	<webwork source="Library/PCC/BasicAlgebra/AlgebraicProperties/ExpressionAlgebraSkill50.pg"/>
</p>

<p>
	4. <webwork source="Library/Mizzou/Algebra/exponents_rational/conv_exp_to_exp_two_term_div_02.pg" />
</p>


<p>
	5. <webwork source="Library/LoyolaChicago/Precalc/Chap3Tools/Connally3-3-Tools-32.pg" />
</p>
	
<p>
	6. <webwork source="Library/LoyolaChicago/Precalc/Chap3Tools/Connally3-3-Tools-46.pg" />
</p>

<p>
	7. <webwork source="Library/UMN/algebraKaufmannSchwitters/ks_5_1_30.pg" />
</p>

<p>
	8. <webwork source="Library/FortLewis/Basic-skills-pretest/Skill-Assessment-06.pg" />
</p>

<p>
	9. <webwork source="Library/UMN/algebraKaufmannSchwitters/ks_5_4_14.pg" />
</p>

<p>
	10. <webwork source="Library/CollegeOfIdaho/setAlgebra_05_06_Factoring/56IntAlg_35_Exponents_Review.pg" />
</p>

<p>
	11. <webwork source="Library/CollegeOfIdaho/setAlgebra_01_06_Exponents/16IntAlg_30_Exponents.pg" />
</p>

<p>
	12. <webwork source="Library/UMN/algebraKaufmannSchwitters/ks_5_2_4.pg" />
</p>

<p>
	13. Note: A monomial is a term of the form <m>ay^b</m> for some constants <m>a</m> and <m>b</m>.  
	
	<webwork source="Library/UMN/algebraKaufmannSchwitters/ks_5_3_24.pg" />
</p>

<p>
	14. <webwork source="Library/UMN/algebraKaufmannSchwitters/ks_5_3_34.pg" />
</p>

<p>
	15. <webwork source="Library/UMN/algebraKaufmannSchwitters/ks_5_4_20.pg" />
</p>
	
<p>
	16. <webwork source="Library/UMN/algebraKaufmannSchwitters/ks_5_4_52.pg" />
</p>

<p>
	17. <webwork source="Library/LoyolaChicago/Precalc/Chap3Tools/Connally3-3-Tools-62.pg" />
</p>

<p>
	18. <webwork source="Library/Mizzou/Algebra/exponents_rational/conv_rad_to_exp_two_term_frac_02.pg" />
</p>

<p>
	19. <webwork source="Library/FortLewis/Algebra/6-2-Fractional-exponents/MCH1-6-2-20-Fractional-exponents.pg" />
</p>

<p>
	20. <webwork source="Library/UMN/algebraKaufmannSchwitters/ks_5_2_46.pg" />
</p>

<p>
	21. <webwork source="Library/Rochester/setAlgebra02ExponentsRadicals/nsc2s7p1.pg" />
</p>
	
<p>
	22. <webwork source="Library/PCC/BasicAlgebra/Exponents/exponentDivision145.pg" />
</p>


<p>
23. <alert> The rest do not seem to render properly...</alert>  <webwork source="Library/Utah/Intermediate_Algebra/set7_Exponential_and_Logarithmic_Functions/s7p17.pg" />
</p>


<p>
9. <webwork source="Library/Utah/Intermediate_Algebra/set7_Exponential_and_Logarithmic_Functions/s7p16.pg" />
</p>

<!--

<p>
10. <webwork source="Library/Utah/Intermediate_Algebra/set14_Review/s14p23.pg" />
</p>

<p>
11. <webwork source="Library/Utah/College_Algebra/set3_Polynomial_and_Rational_Functions/1050s3p7.pg" />
</p>
-->

<!---
<p>
19. <webwork source="Library/LoyolaChicago/Precalc/Chap9Tools/Connally3-9-Tools-28.pg" />
</p>

<p>
20. <webwork source="Library/ma117DB/set1/srw1_2_11.pg" />
</p>

<p>
21. <webwork source="Library/ma117DB/set1/srw1_2_43.pg" />
</p>

<p>
22. <webwork source="Library/Rochester/setAlgebra02ExponentsRadicals/sw1_3_25.pg" />
</p>
-->

<!---
<p>
25. <webwork source="Library/Mizzou/Algebra/radicals_simplifying/two_rad_fractions_03.pg" />
</p>
--> 

</subsection>
</section>